Benchmarks.lean
@@ -2,3 +2,4 @@ import Benchmarks.WETH9.Correct
 import Benchmarks.GnosisMultiSig.Correct
 import Benchmarks.Safe.Correct
 import Benchmarks.UniswapV3Pool.Correct
+import Benchmarks.Dss.Dai.Correct
